HMAC_spec_concat.v
@@ -6,13 +6,16 @@ Require Import HMAC_common_defs.
 Require Import SHA256.
 Require Import HMAC_spec_pad.
 Require Import Coq.Program.Basics.
+Require Import Coqlib.
+Require Import ByteBitRelations.
+Require Import sha_padding_lemmas.
 
 Module HMAC_Concat.
 
 Section HMAC.
 
   Variable c p : nat.
-  Definition b := c + p.
+  Definition b := (c + p)%nat.
   
   (* The compression function *)
   Variable h : Blist -> Blist -> Blist.
@@ -23,7 +26,7 @@ Section HMAC.
 
   (* The iteration of the compression function gives a keyed hash function on lists of words. *)
   Definition h_star k (m : Blist) :=
-    hash_blocks_bits h m k.
+    hash_blocks_bits h k m.
   (* The composition of the keyed hash function with the IV gives a hash function on lists of words. *)
   Definition hash_words := h_star iv.
 
@@ -68,17 +71,96 @@ End HMAC.
 
 End HMAC_Concat.
 
-Check HMAC_Concat.HMAC.
-Check HMAC_Pad.HMAC.
 
-(* TODO fill these in *)
-(* TODO move splitAndPad to HMAC_common *)
-Parameter splitAndPad : Blist -> Blist.
-Parameter fpad : Blist -> Blist.
+Lemma h_star_eq :
+  HMAC_Pad.h_star = HMAC_Concat.h_star.
+Proof. reflexivity. Qed.
+
+(* TODO add assumptions, prove, prove assumptions where used, and move to ByteBitRelations *)
+
+Lemma bitsToBytes_len : forall (l : Blist),
+                          True ->
+                          Zlength (bitsToBytes l) = BlockSize.
+Proof.
+
+Admitted.
+
+Lemma bitsToBytes_app : forall (l m : Blist),
+                          True ->
+                          True ->
+                          bitsToBytes (l ++ m) = bitsToBytes l ++ bitsToBytes m.
+Proof.
+
+Admitted.
+
+Lemma bits_bytes_bits_id : forall (l : Blist),
+                             True ->
+                             bytesToBits (bitsToBytes l) = l.
+Proof.
+
+Admitted.
+
+Lemma splitandpad_eq : forall (l m : Blist),
+                         length l = b ->
+                         (* TODO m is InBlocks *)
+                         sha_splitandpad (l ++ m) = l ++ sha_splitandpad_inc m.
+Proof.
+  intros l m len.
+  unfold sha_splitandpad. unfold sha_splitandpad_inc.
+  unfold pad. unfold pad_inc.
+
+  rewrite -> bitsToBytes_app.
+  rewrite -> common_lemmas.Zlength_app.
+  repeat rewrite -> bytesToBits_app.
+  rewrite -> bits_bytes_bits_id.
+  rewrite <- app_assoc.
+  repeat f_equal.
+  unfold c, p, b in *.
+
+  apply bitsToBytes_len.
+    admit.
+  apply bitsToBytes_len.
+    admit.
+  apply bitsToBytes_len.
+    admit.
+  admit.
+  admit.
+  admit.
+Qed.
+
+Lemma fpad_eq : forall (l m : Blist),
+                  length l = b ->
+                  (* TODO m is in blocks *)
+                  sha_splitandpad (l ++ m) = l ++ HMAC_Concat.app_fpad fpad m.
+Proof.
+  intros l m len.
+  unfold HMAC_Concat.app_fpad.
+  unfold sha_splitandpad. unfold fpad.
+  unfold pad. unfold fpad_inner.
+
+  rewrite -> bitsToBytes_app.
+  repeat rewrite -> bytesToBits_app.
+  repeat rewrite -> bits_bytes_bits_id.
+  rewrite <- app_assoc.
+  rewrite -> common_lemmas.Zlength_app.
+  repeat f_equal.
+
+  apply bitsToBytes_len.
+    admit.
+  apply bitsToBytes_len.
+    admit.
+  apply bitsToBytes_len.
+    admit.
+  admit.
+  admit.
+  admit.
+  admit.
+Qed. 
 
 Theorem HMAC_concat_pad : forall (k m : Blist) (op ip : Blist),
+                            (* TODO length guarantees on k, ip, and op *)
   HMAC_Pad.HMAC c p sha_h sha_iv sha_splitandpad op ip k m =
-  HMAC_Concat.HMAC c p sha_h sha_iv splitAndPad fpad op ip k m.
+  HMAC_Concat.HMAC c p sha_h sha_iv sha_splitandpad_inc fpad op ip k m.
 Proof.
   intros k m op ip.
   unfold c, p in *. simpl in *.
@@ -87,13 +169,23 @@ Proof.
   unfold HMAC_Pad.GHMAC_2K. unfold HMAC_Concat.GHMAC_2K.
 
   repeat rewrite -> split_append_id.
-  unfold HMAC_Pad.hash_words_padded.
+  unfold HMAC_Pad.hash_words_padded. unfold compose.
   unfold HMAC_Concat.hash_words.
-  unfold HMAC_Concat.app_fpad.
-  unfold compose.
+  unfold HMAC_Pad.hash_words.
+  rewrite -> h_star_eq.
   
-  
+  (* show the two inputs to h_star are equal *)
+  f_equal.
 
+  rewrite <- splitandpad_eq.
+  rewrite <- fpad_eq.
+  reflexivity.
 
-Admitted.
-
+(* TODO split out lemma that BLxor preserves length given 2 of block size *)
+  admit.
+  admit.
+  admit.
+  admit.
+  admit.
+  admit.
+Qed.
